Adapt suggestions for proof

proof/Timing_Function_Analysis.thy
@@ -8,8 +8,8 @@ text \<open>Formalization of David Sands' "Calculi for time analysis of function
       Chapter 2 "Computational-Models and Cost-Functions"\<close>
 
 text \<open>Assuming the model to works under natural numbers.\<close>
-typedecl typs
-datatype val = N nat | Ty typs
+typedecl "value"
+datatype val = N nat | V "value"
 fun val_to_nat :: "val \<Rightarrow> nat" where
   "val_to_nat (N n) = n"
 
@@ -17,23 +17,23 @@ definition false :: "val \<Rightarrow> bool" where "false v \<equiv> v = N 0"
 definition true :: "val \<Rightarrow> bool" where "true v \<equiv> \<not> false v"
 
 text \<open>Definition of functions and primary functions\<close>
-datatype func =
-  Func string     ("($_)")
-| cFunc func    ("(c$_)")
-datatype pfunc = pFunc string   ("(p$_)")
+datatype funId =
+  Fun string
+| cFun string
+datatype pfunId = pFun string
 
 text \<open>Defines simple expression\<close>
 datatype exp =
-    App func "exp list"         ("(_/> _)")
-  | pApp pfunc "exp list"       ("(_/: _)")
+    App "funId" "exp list"      (infix "$" 100)
+  | pApp pfunId "exp list"      (infix "$$" 100)
   | If exp exp exp              ("(IF _/ THEN _/ ELSE _)")
-  | Ident nat                   ("(i#_)")
-  | Const val                   ("(c#_)")
+  | Ident nat
+  | Const val
 
 text \<open>env represents local variables in a expression / function\<close>
 type_synonym env = "val list"
 text \<open>defs contains all the functions defined\<close>
-type_synonym defs = "func \<Rightarrow> exp option"
+type_synonym defs = "funId \<Rightarrow> exp option"
 
 text \<open>Exact set of primitive functions is unspecified,
       Sand assumes arithmetic and boolean functions as well as list constructor.
@@ -41,32 +41,27 @@ text \<open>Exact set of primitive functions is unspecified,
 axiomatization pApp :: "string \<Rightarrow> val list \<Rightarrow> val" where
   sum: "pApp ''sum'' es = (N o sum_list o map val_to_nat) es"
 
-text \<open>The syntax \<rho> \<turnstile>\<phi> e \<rightarrow> v reads as
+text \<open>The syntax \<rho>, \<phi> \<turnstile> e \<rightarrow> v reads as
   "Given environment \<rho>, in the context of definitions \<phi> expression e evaluates to value v"\<close>
-inductive eval :: "env \<Rightarrow> defs \<Rightarrow> exp \<Rightarrow> val \<Rightarrow> bool" ("(_/ \<turnstile>_/ _/ \<rightarrow> _)") where
-Id:   "\<rho> \<turnstile>\<phi> i#i \<rightarrow> (\<rho> ! i)" |
-C:    "\<rho> \<turnstile>\<phi> c#v \<rightarrow> v" |
-F:    "length es = length vs \<Longrightarrow> (\<forall>i < length vs. \<rho> \<turnstile>\<phi> (es ! i) \<rightarrow> (vs ! i))
-        \<Longrightarrow> \<phi> f = Some fe \<Longrightarrow> vs \<turnstile>\<phi> fe \<rightarrow> v \<Longrightarrow> \<rho> \<turnstile>\<phi> (f> es) \<rightarrow> v" |
-P:    "length es = length vs \<Longrightarrow> (\<forall>i < length es. \<rho> \<turnstile>\<phi> (es ! i) \<rightarrow> (vs ! i))
-        \<Longrightarrow> pApp p vs = v \<Longrightarrow> \<rho> \<turnstile>\<phi> (p$p: es) \<rightarrow> v" |
-If1:  "\<rho> \<turnstile>\<phi> b \<rightarrow> v \<Longrightarrow> true v \<Longrightarrow> \<rho> \<turnstile>\<phi> t \<rightarrow> et \<Longrightarrow> \<rho> \<turnstile>\<phi> (IF b THEN t ELSE f) \<rightarrow> et" |
-If2:  "\<rho> \<turnstile>\<phi> b \<rightarrow> v \<Longrightarrow> false v \<Longrightarrow> \<rho> \<turnstile>\<phi> f \<rightarrow> ef \<Longrightarrow> \<rho> \<turnstile>\<phi> (IF b THEN t ELSE f) \<rightarrow> ef"
+inductive eval :: "env \<Rightarrow> defs \<Rightarrow> exp \<Rightarrow> val \<Rightarrow> bool" ("(_/, _/ \<turnstile>_/ \<rightarrow> _)") where
+Id:   "\<rho>, \<phi> \<turnstile> Ident i \<rightarrow> (\<rho> ! i)" |
+C:    "\<rho>, \<phi> \<turnstile> Const v \<rightarrow> v" |
+F:    "length es = length vs \<Longrightarrow> (\<forall>i < length vs. \<rho>, \<phi> \<turnstile> (es ! i) \<rightarrow> (vs ! i))
+        \<Longrightarrow> \<phi> f = Some fe \<Longrightarrow> vs, \<phi> \<turnstile> fe \<rightarrow> v \<Longrightarrow> \<rho>, \<phi> \<turnstile> (f$ es) \<rightarrow> v" |
+P:    "length es = length vs \<Longrightarrow> (\<forall>i < length es. \<rho>, \<phi> \<turnstile> (es ! i) \<rightarrow> (vs ! i))
+        \<Longrightarrow> pApp p vs = v \<Longrightarrow> \<rho>, \<phi> \<turnstile> (pFun p$$ es) \<rightarrow> v" |
+If1:  "\<rho>, \<phi> \<turnstile> b \<rightarrow> v \<Longrightarrow> true v \<Longrightarrow> \<rho>, \<phi> \<turnstile> t \<rightarrow> et \<Longrightarrow> \<rho>, \<phi> \<turnstile> (IF b THEN t ELSE f) \<rightarrow> et" |
+If2:  "\<rho>, \<phi> \<turnstile> b \<rightarrow> v \<Longrightarrow> false v \<Longrightarrow> \<rho>, \<phi> \<turnstile> f \<rightarrow> ef \<Longrightarrow> \<rho>, \<phi> \<turnstile> (IF b THEN t ELSE f) \<rightarrow> ef"
 
-inductive_cases IdE[elim!]: "\<rho> \<turnstile>\<phi> i#i \<rightarrow> v"
-inductive_cases CE[elim!]: "\<rho> \<turnstile>\<phi> c#v' \<rightarrow> v"
-inductive_cases FE[elim!]: "\<rho> \<turnstile>\<phi> (f> es) \<rightarrow> v"
-inductive_cases PE[elim!]: "\<rho> \<turnstile>\<phi> (p$p: es) \<rightarrow> v"
-inductive_cases IfE[elim!]: "\<rho> \<turnstile>\<phi> (IF b THEN t ELSE f) \<rightarrow> v"
-declare Id[simp]
-declare C[simp]
-declare F[simp]
-declare P[simp]
-declare If1[simp]
-declare If2[simp]
+inductive_cases IdE[elim!]: "\<rho>, \<phi> \<turnstile> Ident i \<rightarrow> v"
+inductive_cases CE[elim!]: "\<rho>, \<phi> \<turnstile> Const v' \<rightarrow> v"
+inductive_cases FE[elim!]: "\<rho>, \<phi> \<turnstile> (f$ es) \<rightarrow> v"
+inductive_cases PE[elim!]: "\<rho>, \<phi> \<turnstile> (pFun p$$ es) \<rightarrow> v"
+inductive_cases IfE[elim!]: "\<rho>, \<phi> \<turnstile> (IF b THEN t ELSE f) \<rightarrow> v"
+declare eval.intros[simp]
 
 text \<open>Prove that semantic describes deterministic computation\<close>
-proposition "\<lbrakk> \<rho> \<turnstile>\<phi> e \<rightarrow> v; \<rho> \<turnstile>\<phi> e \<rightarrow> v' \<rbrakk> \<Longrightarrow> v = v'"
+proposition "\<lbrakk> \<rho>, \<phi> \<turnstile> e \<rightarrow> v; \<rho>, \<phi> \<turnstile> e \<rightarrow> v' \<rbrakk> \<Longrightarrow> v = v'"
 proof (induction arbitrary: v' rule: eval.induct)
   case (F es vs \<rho> \<phi> f fe v)
   then show ?case
@@ -84,60 +79,53 @@ qed blast+
 
 text \<open>Defines step-counting Semantics.
       Evaluates as eval, but additionally counts the number of applications of non-primitive functions\<close>
-inductive eval_count :: "env \<Rightarrow> defs \<Rightarrow> exp \<Rightarrow> val * nat \<Rightarrow> bool" ("(_/ \<turnstile>_/ _/ \<rightarrow>s _)") where
-cId:   "\<rho> \<turnstile>\<phi> i#i \<rightarrow>s (\<rho>!i,0)" |
-cC:    "\<rho> \<turnstile>\<phi> c#v \<rightarrow>s (v,0)" |
+inductive eval_count :: "env \<Rightarrow> defs \<Rightarrow> exp \<Rightarrow> val * nat \<Rightarrow> bool" ("(_/, _/ \<turnstile> _/ \<rightarrow>s _)") where
+cId:   "\<rho>, \<phi> \<turnstile> Ident i \<rightarrow>s (\<rho>!i,0)" |
+cC:    "\<rho>, \<phi> \<turnstile> Const v \<rightarrow>s (v,0)" |
 cF:    "length es = length vs \<Longrightarrow> length es = length ts
-          \<Longrightarrow> (\<And>i. i < length vs \<Longrightarrow> \<rho> \<turnstile>\<phi> (es!i) \<rightarrow>s (vs!i,ts!i))
-          \<Longrightarrow> \<phi> f = Some fe \<Longrightarrow> vs \<turnstile>\<phi> fe \<rightarrow>s (v,t) \<Longrightarrow> \<rho> \<turnstile>\<phi> (f> es) \<rightarrow>s (v,1+t+sum_list ts)" |
-cP:    "length es = length vs \<Longrightarrow> length es = length ts \<Longrightarrow> (\<And>i. i < length es \<Longrightarrow> \<rho> \<turnstile>\<phi> (es ! i) \<rightarrow>s (vs!i,ts!i))
-          \<Longrightarrow> pApp p vs = v \<Longrightarrow> \<rho> \<turnstile>\<phi> (p$p: es) \<rightarrow>s (v,sum_list ts)" |
-cIf1:  "\<rho> \<turnstile>\<phi> b \<rightarrow>s (eb,tb) \<Longrightarrow> true eb \<Longrightarrow> \<rho> \<turnstile>\<phi> t \<rightarrow>s (et,tt)
-          \<Longrightarrow> \<rho> \<turnstile>\<phi> (IF b THEN t ELSE f) \<rightarrow>s (et,tb+tt)" |
-cIf2:  "\<rho> \<turnstile>\<phi> b \<rightarrow>s (eb,tb) \<Longrightarrow> false eb \<Longrightarrow> \<rho> \<turnstile>\<phi> f \<rightarrow>s (ef,tf)
-          \<Longrightarrow> \<rho> \<turnstile>\<phi> (IF b THEN t ELSE f) \<rightarrow>s (ef,tb+tf)"
+          \<Longrightarrow> (\<And>i. i < length vs \<Longrightarrow> \<rho>, \<phi> \<turnstile> (es!i) \<rightarrow>s (vs!i,ts!i))
+          \<Longrightarrow> \<phi> f = Some fe \<Longrightarrow> vs, \<phi> \<turnstile> fe \<rightarrow>s (v,t) \<Longrightarrow> \<rho>, \<phi> \<turnstile> (f$ es) \<rightarrow>s (v,1+t+sum_list ts)" |
+cP:    "length es = length vs \<Longrightarrow> length es = length ts \<Longrightarrow> (\<And>i. i < length es \<Longrightarrow> \<rho>, \<phi> \<turnstile> (es ! i) \<rightarrow>s (vs!i,ts!i))
+          \<Longrightarrow> pApp p vs = v \<Longrightarrow> \<rho>, \<phi> \<turnstile> (pFun p$$ es) \<rightarrow>s (v,sum_list ts)" |
+cIf1:  "\<rho>, \<phi> \<turnstile> b \<rightarrow>s (eb,tb) \<Longrightarrow> true eb \<Longrightarrow> \<rho>, \<phi> \<turnstile> t \<rightarrow>s (et,tt)
+          \<Longrightarrow> \<rho>, \<phi> \<turnstile> (IF b THEN t ELSE f) \<rightarrow>s (et,tb+tt)" |
+cIf2:  "\<rho>, \<phi> \<turnstile> b \<rightarrow>s (eb,tb) \<Longrightarrow> false eb \<Longrightarrow> \<rho>, \<phi> \<turnstile> f \<rightarrow>s (ef,tf)
+          \<Longrightarrow> \<rho>, \<phi> \<turnstile> (IF b THEN t ELSE f) \<rightarrow>s (ef,tb+tf)"
 
-inductive_cases cIdE[elim!]: "\<rho> \<turnstile>\<phi> i#i \<rightarrow>s v"
-inductive_cases cCE[elim!]: "\<rho> \<turnstile>\<phi> c#v' \<rightarrow>s v"
-inductive_cases cFE[elim!]: "\<rho> \<turnstile>\<phi> (f> es) \<rightarrow>s v"
-inductive_cases cPE[elim!]: "\<rho> \<turnstile>\<phi> (p$p: es) \<rightarrow>s v"
-inductive_cases cIfE[elim!]: "\<rho> \<turnstile>\<phi> (IF b THEN t ELSE f) \<rightarrow>s v"
-declare cId[intro]
-declare cC[intro]
-declare cF[intro]
-declare cP[intro]
-declare cIf1[intro]
-declare cIf2[intro]
+inductive_cases cIdE[elim!]: "\<rho>, \<phi> \<turnstile> Ident i \<rightarrow>s v"
+inductive_cases cCE[elim!]: "\<rho>, \<phi> \<turnstile> Const v' \<rightarrow>s v"
+inductive_cases cFE[elim!]: "\<rho>, \<phi> \<turnstile> (f$ es) \<rightarrow>s v"
+inductive_cases cPE[elim!]: "\<rho>, \<phi> \<turnstile> (pFun p$$ es) \<rightarrow>s v"
+inductive_cases cIfE[elim!]: "\<rho>, \<phi> \<turnstile> (IF b THEN t ELSE f) \<rightarrow>s v"
+declare eval_count.intros[intro]
 
 lemma eval_eval_count':
-  assumes "\<And>i. i < length vs \<Longrightarrow> \<exists>t. \<rho> \<turnstile>\<phi> es ! i \<rightarrow>s (vs ! i, t)"
-  and "length vs = length es"
-  shows  "\<exists>ts. length vs = length ts \<and> (\<forall>i. (i < length vs \<longrightarrow> \<rho> \<turnstile>\<phi> (es!i) \<rightarrow>s (vs!i,ts!i)))"
+  assumes "\<forall>i < length vs. \<exists>t. \<rho>, \<phi> \<turnstile> es ! i \<rightarrow>s (vs ! i, t)"
+  and "length es = length vs"
+  shows  "\<exists>ts. length vs = length ts \<and> (\<forall>i. (i < length vs \<longrightarrow> \<rho>, \<phi> \<turnstile> (es!i) \<rightarrow>s (vs!i,ts!i)))"
   using assms
 proof (induction vs arbitrary: es)
   case (Cons v vs)
   then obtain e e' where e: "(e#e') = es" by (metis length_Suc_conv)
   with Cons(3) have len: "length e' = length vs" by auto
 
-  from Cons(2) e have "\<And>i. i < length (v#vs) \<Longrightarrow> \<exists>t. \<rho> \<turnstile>\<phi> (e#e') ! i \<rightarrow>s ((v#vs) ! i, t)"
-    by blast
-  then have "\<And>i. i < length vs \<Longrightarrow> \<exists>t. \<rho> \<turnstile>\<phi> e' ! i \<rightarrow>s (vs ! i, t)"
+  from Cons(2) e have "\<forall>i < length vs. \<exists>t. \<rho>, \<phi> \<turnstile> e' ! i \<rightarrow>s (vs ! i, t)"
     by fastforce
-  with Cons(1) len
-  obtain ts where ts: "length vs = length ts" "\<forall>i<length vs. \<rho> \<turnstile>\<phi> e' ! i \<rightarrow>s (vs ! i, ts ! i)"
-    by metis
-  from Cons(2) obtain t where t: "\<rho> \<turnstile>\<phi> (es ! 0) \<rightarrow>s ((v # vs) ! 0,t)" by blast
+  from Cons(1)[OF this len]
+  obtain ts where ts: "length vs = length ts" "\<forall>i<length vs. \<rho>, \<phi> \<turnstile> e' ! i \<rightarrow>s (vs ! i, ts ! i)"
+    by blast
+  from Cons(2) obtain t where t: "\<rho>, \<phi> \<turnstile> (es ! 0) \<rightarrow>s ((v # vs) ! 0,t)" by blast
 
   have "length (v#vs) = length (t#ts)" using len ts by simp
   moreover
-  have "\<forall>i<length (v#vs). \<rho> \<turnstile>\<phi> es ! i \<rightarrow>s ((v#vs) ! i, (t#ts) ! i)"
-    using ts t e
+  have "\<forall>i<length (v#vs). \<rho>, \<phi> \<turnstile> es ! i \<rightarrow>s ((v#vs) ! i, (t#ts) ! i)"
+    using ts(2) t e
     by (metis Suc_less_eq length_Cons not0_implies_Suc nth_Cons_0 nth_Cons_Suc)
 
   ultimately show ?case by blast
 qed simp
 
-lemma eval_eval_count: "\<rho> \<turnstile>\<phi> b \<rightarrow> v \<Longrightarrow> \<exists>t. \<rho> \<turnstile>\<phi> b \<rightarrow>s (v,t)"
+lemma eval_eval_count: "\<rho>, \<phi> \<turnstile> b \<rightarrow> v \<Longrightarrow> \<exists>t. \<rho>, \<phi> \<turnstile> b \<rightarrow>s (v,t)"
 proof (induction rule: eval.induct)
   case (F es vs \<rho> \<phi> f fe v)
   then show ?case
@@ -148,76 +136,75 @@ next
     by (metis cP eval_eval_count')
 qed blast+
 
-lemma eval_count_eval: "\<rho> \<turnstile>\<phi> b \<rightarrow>s (v,t) \<Longrightarrow> \<rho> \<turnstile>\<phi> b \<rightarrow> v"
+lemma eval_count_eval: "\<rho>, \<phi> \<turnstile> b \<rightarrow>s (v,t) \<Longrightarrow> \<rho>, \<phi> \<turnstile> b \<rightarrow> v"
   by (induction \<rho> \<phi> b "(v,t)" arbitrary: v t rule: eval_count.induct) auto
 
 text \<open>Show that computation result of eval and eval_count is equal\<close>
-theorem  eval_eq_eval_count: "(\<rho> \<turnstile>\<phi> b \<rightarrow> v) \<longleftrightarrow> (\<exists>t. \<rho> \<turnstile>\<phi> b \<rightarrow>s (v,t))"
+theorem  eval_eq_eval_count: "(\<rho>, \<phi> \<turnstile> b \<rightarrow> v) \<longleftrightarrow> (\<exists>t. \<rho>, \<phi> \<turnstile> b \<rightarrow>s (v,t))"
   using eval_count_eval eval_eval_count by auto
 
 text \<open>\<T> constructs the cost function for an expression\<close>
 fun \<T> :: "exp \<Rightarrow> exp" where
-  "\<T> c#v = c#N 0"
-| "\<T> i#i = c#N 0"
-| "\<T> (IF b THEN t ELSE f) = p$''sum'': [\<T> b, IF b THEN \<T> t ELSE \<T> f]"
-| "\<T> (p$_: args) = p$''sum'': map \<T> args"
-| "\<T> (f> args) = p$''sum'': (c$f> args # map \<T> args)"
+  "\<T> (Const v) = Const (N 0)"
+| "\<T> (Ident i) = Const (N 0)"
+| "\<T> (IF b THEN t ELSE f) = pFun ''sum''$$ [\<T> b, IF b THEN \<T> t ELSE \<T> f]"
+| "\<T> (pFun _$$ args) = pFun ''sum''$$ map \<T> args"
+| "\<T> (Fun f$ args) = pFun ''sum''$$ (cFun f$ args # map \<T> args)"
+| "\<T> (cFun f$ args) = pFun ''sum''$$ (cFun f$ args # map \<T> args)"
 
-text \<open>c constructs the cost function for a function given by its expression\<close>
-fun c :: "exp \<Rightarrow> exp" where
-  "c e = p$''sum'': [c#N 1, \<T> e]"
+text \<open>cost constructs the cost function for a function given by its expression\<close>
+definition cost :: "exp \<Rightarrow> exp" where
+  "cost e = pFun ''sum''$$ [Const (N 1), \<T> e]"
 
 text \<open>Adds cost functions for existing functions in a definition\<close>
 fun conv :: "defs \<Rightarrow> defs" where
-  "conv \<phi> (c$f) = (case \<phi> f of None \<Rightarrow> None | Some e \<Rightarrow> Some (c e))"
-| "conv \<phi> ($f) = \<phi> $f"
+  "conv \<phi> (Fun f) = \<phi> (Fun f)"
+| "conv \<phi> (cFun f) = (case \<phi> (Fun f) of None \<Rightarrow> None | Some e \<Rightarrow> Some (cost e))"
 
-text \<open>A definition is correct if each cost function fits to its function\<close>
-definition defs_cor where
-  "defs_cor \<phi> =
-  (\<forall>f. (case \<phi> f of Some e \<Rightarrow> \<phi> (c$f) = None \<or> \<phi> (c$f) = Some (c e)
-                  | None \<Rightarrow> \<phi> (c$f) = None))"
+text \<open>Defines premise for definitions without timing functions\<close>
+definition no_time where
+  "no_time \<phi> = (\<forall>f. \<phi> (cFun f) = None)"
 
-lemma conv_trans: "defs_cor \<phi> \<Longrightarrow> \<phi> f = Some e \<Longrightarrow> (conv \<phi>) f = Some e"
-  apply (induction f arbitrary: e)
-  by auto (smt (verit, del_insts) case_optionE defs_cor_def option.case_eq_if option.distinct(1))
-
-lemma eval_conv_trans: "\<rho> \<turnstile>\<phi> e \<rightarrow> v \<Longrightarrow> defs_cor \<phi> \<Longrightarrow> \<rho> \<turnstile>(conv \<phi>) e \<rightarrow> v"
-  by (induction rule: eval.induct) (auto simp: conv_trans)
+lemma no_time_trans: "no_time \<phi> \<Longrightarrow> \<phi> f = Some e \<Longrightarrow> (conv \<phi>) f = Some e"
+  by (induction f arbitrary: e) (auto simp: no_time_def)
+lemma eval_no_time_trans: "\<rho>, \<phi> \<turnstile> e \<rightarrow> v \<Longrightarrow> no_time \<phi> \<Longrightarrow> \<rho>, (conv \<phi>) \<turnstile> e \<rightarrow> v"
+  by (induction rule: eval.induct) (auto simp: no_time_trans)
 
 text \<open>Prove correctness theorem that the converted expression with converted definitions
       evaluates to the same result as the evaluated by the step counting semantic\<close>
 theorem conv_cor:
-  assumes "\<rho> \<turnstile>\<phi> e \<rightarrow>s (s,t)"
-    and   "defs_cor \<phi>"
-   shows  "\<rho> \<turnstile>(conv \<phi>) (\<T> e) \<rightarrow> N t"
+  assumes "\<rho>, \<phi> \<turnstile> e \<rightarrow>s (s,t)"
+    and   "no_time \<phi>"
+   shows  "\<rho>, (conv \<phi>) \<turnstile> (\<T> e) \<rightarrow> N t"
   using assms
 proof (induction \<rho> \<phi> e "(s,t)" arbitrary: s t rule: eval_count.induct)
   case (cF es vs ts \<rho> \<phi> f fe v t)
+
+  from cF(5) cF(8)
+  obtain fn where f_fn: "f = Fun fn"
+    by (cases f) (auto simp: no_time_def)
 
   obtain ts' where ts: "ts' = map N ts" by simp
   then have papp: "pApp ''sum'' (N (1 + t) # ts') = N (1 + t + sum_list ts)"
     by (simp add: comp_def sum)
   
-  from P[of "[c#N 1, \<T> fe]" "[N 1,N t]" vs "conv \<phi>" "''sum''" "N (1+t)"] cF.hyps(7) cF.prems sum
-  have "vs \<turnstile>conv \<phi> p$''sum'': [c#N 1, \<T> fe] \<rightarrow> N (1 + t)"
+  from P[of "[Const (N 1), \<T> fe]" "[N 1,N t]" vs "conv \<phi>" "''sum''" "N (1+t)"] cF.hyps(7)[OF cF.prems] sum
+  have c_fe: "vs, conv \<phi> \<turnstile> cost fe \<rightarrow> N (1 + t)"
+    by (simp add: nth_Cons' cost_def)
+
+  from cF.hyps(3) eval_no_time_trans[OF _ cF.prems] eval_eq_eval_count
+  have "\<forall>i<length vs. \<rho>, conv \<phi> \<turnstile> es ! i \<rightarrow> vs ! i" by blast
+
+  with cF(1) cF(5) c_fe f_fn
+  have "\<rho>, conv \<phi> \<turnstile> cFun fn$ es \<rightarrow> N (1 + t)" by simp
+
+  with cF.hyps(1) cF.hyps(4)[OF _ cF.prems] ts cF.hyps(2)
+  have "\<forall>i<length (cFun fn$ es # map \<T> es). \<rho>, conv \<phi> \<turnstile> (cFun fn$ es # map \<T> es) ! i \<rightarrow> ((N (1 + t)) # ts') ! i"
     by (simp add: nth_Cons')
-  then have c_fe: "vs \<turnstile>conv \<phi> (c fe) \<rightarrow> N (1 + t)" by simp
 
-  from cF.hyps(3) cF.prems eval_conv_trans eval_eq_eval_count
-  have "\<forall>i<length vs. \<rho> \<turnstile>conv \<phi> es ! i \<rightarrow> vs ! i" by blast
-
-  with cF(1) cF(5) c_fe F[of es vs \<rho> "conv \<phi>" "c$f" "c fe" "N (1+t)"]
-  have "\<rho> \<turnstile>conv \<phi> c$f> es \<rightarrow> N (1 + t)" by simp
-
-  with cF.hyps(1) cF.hyps(4) cF.prems ts cF.hyps(2)
-  have "\<forall>i<length (c$f> es # map \<T> es). \<rho> \<turnstile>conv \<phi> (c$f> es # map \<T> es) ! i \<rightarrow> ((N (1 + t)) # ts') ! i"
-    by (simp add: nth_Cons')
-
-  with cF.hyps(2) sum papp ts
-    P[of "c$f> es # map \<T> es" "(N (1+t)) # ts'" \<rho> "conv \<phi>" "''sum''" "N (1 + t + sum_list ts)"]
-  show ?case
-    by simp
+  from cF.hyps(2) sum ts f_fn
+    P[OF _ this papp]
+  show ?case by simp
 next
   case (cP es vs ts \<rho> \<phi> p v)
   
@@ -225,68 +212,34 @@ next
   then have papp: "pApp ''sum'' ts' = N (sum_list ts)"
     by (simp add: comp_def sum)
 
-  with ts cP sum P[of "map \<T> es" ts' \<rho> "conv \<phi>" "''sum''" "(N o sum_list o map val_to_nat) ts'"(*"map val_to_nat ts" \<rho> "conv \<phi>" "''sum''" "(sum_list) ts"*)]
-  show ?case
-    by simp
+  with ts cP(2) cP(4)[OF _ cP(6)] sum P[of "map \<T> es" ts' \<rho> "conv \<phi>" "''sum''" "(N o sum_list o map val_to_nat) ts'"]
+  show ?case by simp
 next
   case (cIf1 \<rho> \<phi> b eb tb t et tt f)
 
   let ?ts = "[\<T> b, IF b THEN \<T> t ELSE \<T> f]"
 
-  have "\<rho> \<turnstile>\<phi> b \<rightarrow> eb"
-    using cIf1(1) eval_count_eval by auto
-
-  then have b: "\<rho> \<turnstile>(conv \<phi>) b \<rightarrow> eb"
-    using cIf1.prems eval_conv_trans by auto
-
-  from b cIf1(3) cIf1(5)
-  have ifelse: "\<rho> \<turnstile>(conv \<phi>) IF b THEN \<T> t ELSE \<T> f \<rightarrow> N tt"
-    by (simp add: cIf1.prems)
-
-  from cIf1(2) ifelse
-  have args: "(\<forall>i < length ?ts. \<rho> \<turnstile>(conv \<phi>) (?ts ! i) \<rightarrow> ([N tb,N tt] ! i))"
-    by (simp add: cIf1.prems nth_Cons')
+  from cIf1(2)[OF cIf1.prems]
+    If1[OF eval_no_time_trans[OF eval_count_eval[OF cIf1(1)] cIf1.prems] cIf1(3) cIf1(5)[OF cIf1.prems]]
+  have args: "(\<forall>i < length ?ts. \<rho>, conv \<phi> \<turnstile> (?ts ! i) \<rightarrow> ([N tb,N tt] ! i))"
+    by (simp add: nth_Cons')
   have app: "pApp ''sum'' [N tb,N tt] = N (tb + tt)" by (simp add: sum)
 
-  from args app P[of ?ts "[N tb,N tt]"]
-  have "\<rho> \<turnstile>conv \<phi> (p$''sum'': ?ts) \<rightarrow> N (tb + tt)" by simp
-  then show ?case by simp
+  from sum P[OF _ args app]
+  show ?case by simp
 next
   case (cIf2 \<rho> \<phi> b eb tb f ef tf t)
 
   let ?ts = "[\<T> b, IF b THEN \<T> t ELSE \<T> f]"
 
-  have "\<rho> \<turnstile>\<phi> b \<rightarrow> eb"
-    using cIf2(1) eval_count_eval by auto
-
-  then have b: "\<rho> \<turnstile>(conv \<phi>) b \<rightarrow> eb"
-    using cIf2.prems eval_conv_trans by auto
-
-  from b cIf2(3) cIf2(5)
-  have ifelse: "\<rho> \<turnstile>(conv \<phi>) IF b THEN \<T> t ELSE \<T> f \<rightarrow> N tf"
-    by (simp add: cIf2.prems)
-
-  from cIf2(2) ifelse
-  have args: "(\<forall>i < length ?ts. \<rho> \<turnstile>(conv \<phi>) (?ts ! i) \<rightarrow> ([N tb,N tf] ! i))"
-    by (simp add: cIf2.prems nth_Cons')
+  from cIf2(2)[OF cIf2.prems]
+    If2[OF eval_no_time_trans[OF eval_count_eval[OF cIf2(1)] cIf2.prems] cIf2(3) cIf2(5)[OF cIf2.prems]]
+  have args: "(\<forall>i < length ?ts. \<rho>, conv \<phi> \<turnstile> (?ts ! i) \<rightarrow> ([N tb,N tf] ! i))"
+    by (simp add: nth_Cons')
   have app: "pApp ''sum'' [N tb,N tf] = N (tb + tf)" by (simp add: sum)
 
-  from args app P[of ?ts "[N tb,N tf]"]
-  have "\<rho> \<turnstile>conv \<phi> (p$''sum'': ?ts) \<rightarrow> N (tb + tf)" by simp
-  then show ?case by simp
+  from sum P[OF _ args app]
+  show ?case by simp
 qed simp+
-
-text \<open>Defines a simple variant of correct definitions: no existing timing functions\<close>
-definition no_time where
-  "no_time \<phi> = (\<forall>f. \<phi> c$f = None)"
-
-lemma no_time_defs_cor: "no_time \<phi> \<Longrightarrow> defs_cor \<phi>"
-  by (simp add: defs_cor_def no_time_def option.case_eq_if)
-
-corollary conv_cor_no_time:
-  assumes "\<rho> \<turnstile>\<phi> e \<rightarrow>s (s,t)"
-    and   "no_time \<phi>"
-   shows  "\<rho> \<turnstile>(conv \<phi>) (\<T> e) \<rightarrow> N t"
-  using assms conv_cor no_time_defs_cor by auto
 
 end
